proof of pmac

casestudy/openSSL/pmac_verify_hmac/pmac_verify_hmac_proof_BL_CL32.ec
@@ -18,54 +18,93 @@ proof.
 qed.
 
 op inv (j off i:W64.t) = 
-   if to_uint j < to_uint off then to_uint i = 0
-  else if to_uint j < to_uint off + 20 then to_uint i = to_uint j - to_uint off
+   if to_sint j < to_sint off then to_uint i = 0
+  else if to_sint j < to_sint off + 20 then to_uint i = to_sint j - to_sint off
   else to_uint i = 20.
 
-lemma inv_incr j off i : 
-  W64.to_uint j < 276 => 
+lemma to_sintD_small (x y : W64.t): 
+  W64.min_sint <= to_sint x + to_sint y <= W64.max_sint =>
+  to_sint (x + y) = to_sint x + to_sint y.
+proof. rewrite /W64.to_sint /smod W64.to_uintD /#. qed.
+
+lemma to_sintB_small (x y : W64.t) : 
+  W64.min_sint <= to_sint x - to_sint y <= W64.max_sint =>
+  to_sint (x - y) = to_sint x - to_sint y.
+proof. rewrite /W64.to_sint /smod W64.to_uintD to_uintNE !modzDmr /= /#. qed.
+
+lemma to_sint_small (x:int) :
+  W64.min_sint <= x <= W64.max_sint =>
+  to_sint (W64.of_int x) = x.
+proof. rewrite /to_sint /smod W64.of_uintK /= /#. qed.
+
+lemma inv_incr (len  maxpad off j i: W64.t):
+  to_uint maxpad <= 276 => 
+  to_uint len <= to_uint maxpad + 1 =>
+  off = (maxpad+ W64.one) - len => 
+  W64.to_uint j < to_uint maxpad => 
   inv j off i =>
   inv (j + W64.one) off
     (i + invw (invw (j - off - W64.of_int 20 `|>>` W8.of_int 63)) `&` (off - W64.one - j `|>>` W8.of_int 63) `&` W64.one).
 proof.
   rewrite !invwK /W64.(`|>>`) W8.to_uint_small 1:// modz_small 1://.
-  rewrite !sar_and /inv => /> hj.
-  rewrite (W64.to_uintD_small j W64.one) 1:/#.
-  have -> : to_sint (j - off - W64.of_int 20) = to_uint j - to_uint off - 20.
-  + admit.
-  have heq : to_sint (off - W64.one - j) = to_uint off - 1 - to_uint j.
-  + admit.
-  case: (to_uint j < to_uint off) => hjoff /=.
-  + move=> hi; have -> /= : to_uint j - to_uint off - 20 < 0 by smt().
-    by rewrite sar_and heq; have -> /= /#: !(to_uint off - 1 - to_uint j < 0) by smt().
-  case: (to_uint j < to_uint off + 20) => hjoff20.
-  + have -> /= :  to_uint j - to_uint off - 20 < 0 by smt().
+  rewrite !sar_and /inv => hm hl hoff hj.
+  have sulen : to_sint len = to_uint len by rewrite /to_sint /smod /#. 
+  have suj : to_sint j = to_uint j by rewrite /to_sint /smod /#. 
+  have sumax : to_sint maxpad = to_uint maxpad by rewrite /to_sint /smod /#. 
+  have /= ?:= W64.to_uint_cmp j; have /= ?:= W64.to_uint_cmp maxpad; have /= ?:= W64.to_uint_cmp len.
+  have h1 := to_sint_small 1 _; 1 : done.
+  rewrite (to_sintD_small j W64.one) h1; 1: by rewrite /= /#.
+  have hoff' : to_sint off = (to_sint maxpad + 1) - to_sint len.
+  + by rewrite hoff to_sintB_small to_sintD_small /to_sint /smod /= // /#.
+  have -> : to_sint (j - off - W64.of_int 20) = to_sint j - to_sint off - 20.
+  + have -> : j - off - W64.of_int 20 = j - (off + W64.of_int 20) by ring.
+    have h : to_sint (off + W64.of_int 20) = to_sint off + 20.
+    + by rewrite to_sintD_small ?to_sint_small // hoff to_sintB_small to_sintD_small /= /to_sint /smod /=; smt(). 
+    rewrite to_sintB_small h hoff'; 2: by ring.
+    by rewrite /to_sint /smod /=; smt().
+  have heq : to_sint (off - W64.one - j) = to_sint off - 1 - to_sint j.
+  + have -> : off - W64.one - j = off - (W64.one + j) by ring.
+    have h : to_sint (W64.one + j) = to_sint j + 1.
+    + by rewrite to_sintD_small ?to_sint_small // /= /to_sint /smod /=; smt(). 
+    by rewrite to_sintB_small h /= /#.
+  case: (to_sint j < to_sint off) => hjoff /=.
+  + move=> hi; have -> /= : to_sint j - to_sint off - 20 < 0 by smt().
+    by rewrite sar_and heq; have -> /= /#: !(to_sint off - 1 - to_sint j < 0) by smt().
+  case: (to_sint j < to_sint off + 20) => hjoff20.
+  + have -> /= :  to_sint j - to_sint off - 20 < 0 by smt().
     rewrite sar_and heq => hi.
-    split => hj1.
-    + by have -> /= : !(to_uint off - 1 - to_uint j < 0); smt().
-    case: (to_uint off - 1 - to_uint j < 0) => hoff1j /=.
-    + by rewrite (W64.to_uintD_small i W64.one) /= /#.
-    smt().    
-  have -> /= : !(to_uint j - to_uint off - 20 < 0); smt().
+    have -> /= : !(to_sint j + 1 < to_sint off) by smt().
+    have -> /= : to_sint off - 1 - to_sint j < 0 by smt().
+    by rewrite W64.to_uintD_small /= /#. 
+  have -> /= : !(to_sint j + 1 < to_sint off) by smt().
+  have -> /= : !(to_sint j + 1 < to_sint off + 20) by smt().
+  have -> // : !(to_sint j - to_sint off - 20 < 0) by smt().
 qed.
 
 equiv l_final : M.verify_hmac_jazz ~ M.verify_hmac_jazz :
-  ={M.leakages, len, pmac, out, maxpad} /\ to_uint pmac{2} + 32 <= W64.modulus /\ 32 %| to_uint pmac{2} /\ to_uint maxpad{1} < 256 
-  ==> ={M.leakages}.
+  ={M.leakages, pmac, len, maxpad, out} /\ 
+     to_uint pmac{2} + 32 <= W64.modulus /\ 32 %| to_uint pmac{2} /\ to_uint maxpad{1} < 256  /\
+     (to_uint len <= to_uint maxpad + 21){1} 
+     ==> ={M.leakages}.
 proof.
 proc; wp => /=.
-while (={maxpad, j, p, M.leakages, len, pmac, out, maxpad} /\ 
+while (={maxpad, j, p, M.leakages, len, pmac, maxpad, off} /\ 
        inv j{1} off{1} i{1} /\ inv j{2} off{2} i{2} /\ to_uint j{1} <= to_uint maxpad{1} < 256 + 20 /\ 
-       to_uint pmac{2} + 32 <= W64.modulus /\ 32 %| to_uint pmac{2}).
-+ wp; skip=> |> &1 &2 h1 h2 hjm hmax hpmac dpmac; rewrite ultE => hj.
-  split.
-  + by rewrite /leak_mem /leak_mem_CL32 !offset_div_32 // 1,2:/#.
-  split; 1: by apply inv_incr => //; smt().
-  split; 1: by apply inv_incr => //; smt().
+       to_uint pmac{2} + 32 <= W64.modulus /\ 32 %| to_uint pmac{2} /\ 
+       (off = (maxpad+ W64.one) - len){1} /\ (to_uint len <= to_uint maxpad + 1){1}).
++ wp; skip=> |> &1 &2 h1 h2 hjm hmax hpmac dpmac hlen; rewrite ultE => hj.
+  split; 1: by rewrite /leak_mem /leak_mem_CL32 !offset_div_32 // 1,2:/#.
+  split; 1: by apply (inv_incr len{2} maxpad{2}) => // /#. 
+  split; 1: by apply (inv_incr len{2} maxpad{2}) => // /#. 
   by rewrite (W64.to_uintD_small j{2} W64.one) /#.
-auto => |> &2 hmac dmac hmax.
-rewrite (W64.to_uintD_small maxpad{2}) /= 1:/#.
-have -> : out{2} - (out{2} + len{2} - W64.one - maxpad{2} - W64.of_int 20) = 
-          (W64.one + maxpad{2} + W64.of_int 20) - len{2} by ring.
-rewrite /inv /=; smt(W64.to_uint_cmp).
+auto => |> &1 hpmac dmac hmax hlen.
+rewrite (W64.to_uintD_small maxpad{1}) /= 1:/# hlen /=.
+have -> : out{1} - (out{1} + len{1} - W64.one - maxpad{1} - W64.of_int 20) = 
+          (maxpad{1} + W64.of_int 21) - len{1} by ring.
+have -> /= : inv W64.zero (maxpad{1} + (of_int 21)%W64 - len{1}) W64.zero; last by smt(W64.to_uint_cmp).
+have ? : to_sint (maxpad{1} + (of_int 21)%W64) = to_uint maxpad{1} + 21.
++ rewrite to_sintD_small to_sint_small // /to_sint /smod /=; smt(W64.to_uint_cmp).
+have ? : to_sint len{1} = to_uint len{1} by rewrite /to_sint /smod /=; smt(W64.to_uint_cmp).
+rewrite /inv to_sintB_small /=; 1: smt(W64.to_uint_cmp).
+by rewrite to_sint_small // /#.
 qed.
